managed elim rules

theories/elimRules.v
@@ -50,32 +50,53 @@ Proof.
 Defined.
 
 
-Lemma decidable_and : forall A0, { '(B, C) | A0 = B ∧ C } + { forall B C, A0 <> B ∧ C }.
+
+Ltac s_struct := assert (S = (Γ ⊢? A)) as S_struct; try (destruct S; reflexivity).
+
+Definition Q_and (A : formula)  (l0 : list formula) (A0 : formula) (l1 : list formula) :=
+ (forall B C, A0 = B ∧ C -> notT (l0 ++ [B;C] ++ l1 ⊢ A)).
+
+Lemma f_and : forall  l0 A0 l1, l0 ++ [A0] ++ l1= Γ -> (Γ ⊢ A) + {Q_and A l0 A0 l1}.
 Proof.
-  intro A0.
-  induction A0.
-  - right. intros B C N. inversion N.
-  - right. intros B C N. inversion N.
-  - right. intros B C N. inversion N.
-  - left. exists (A0_1,A0_2). reflexivity.
-  - right. intros B C N. inversion N.
-  - right. intros B C N. inversion N.
+  intros l0 A0 l1 eq.
+
+  unfold Q_and.
+  specialize (decidable_and A0) as [[[B C] eq0] | Neg].
+  - 
+    specialize (deg_IE_and l0 B C l1 A) as Deg.
+    rewrite eq0 in eq.
+    rewrite <- eq in IH.
+    apply IH in Deg.
+    destruct Deg as [L | R].
+    + rewrite <- eq.
+      left.
+      apply IE_and.
+      assumption.
+    + right.
+      destruct S.
+      intros B0 C0 H.
+      rewrite H in eq0.
+      inversion eq0.
+      subst.
+      assumption.
+  - right.
+    destruct S.
+    intros B C H N.
+    specialize (Neg B C).
+    contradiction.
 Defined.
 
-Definition Q_and (l : list formula) (A0 : formula) (r: list formula) := l ++ [A0] ++ r = Γ /\ (forall B C, A0  <> B ∧ C).
-Definition P_and := {'(l,A0,r,B,C) | l ++ [A0] ++ r = Γ   /\  A0 = B ∧ C }.
-
-Lemma either_P_and_or_Q_and : forall l A0 r, l ++ [A0] ++ r = Γ -> P_and + {Q_and l A0 r}.
+Lemma pre_IE_and : (Γ ⊢ A) + {
+      forall l0 A0 l1, l0 ++ [A0] ++ l1 = Γ -> Q_and A l0 A0 l1}.
 Proof.
-  intros l A0 r H.
-  unfold P_and, Q_and.
-  specialize (decidable_and A0) as [[[B C] eq] | Neq].
-  - left. exists (l, A0, r, B, C). split; assumption.
-  - right. split; assumption.
+  specialize (list_split_ind  formula (Γ ⊢ A)  (Q_and A) Γ f_and) as [Fine | NotFine].
+  - left. assumption.
+  - right.
+    intros l0 A0 l1 H.
+    apply NotFine.
+    assumption.
 Defined.
-
-
-Ltac dec A B L R:= specialize (formula_eq_dec A B) as [L |  R].
+  
 
 Lemma provable_with_IE_and :
    (Γ ⊢ A) +
@@ -86,36 +107,365 @@ Lemma provable_with_IE_and :
         end
   }.
 Proof.
-  specialize (list_split_ind formula P_and Q_and Γ either_P_and_or_Q_and) as [P_holds | Every_Q_holds].
-  - unfold P_and in P_holds.
-    destruct P_holds as [[[[[l A0] r] B] C] [eq_Γ eq_A0]].
-    subst.
-    specialize (deg_IE_and l B C r A) as Deg.
-    rewrite <- eq_Γ in IH.
-    apply IH in Deg.
-    destruct Deg as [Ok | Bad].
-    + left.
-      rewrite <- eq_Γ.
-      apply IE_and.
+  specialize pre_IE_and as [Done | Workie].
+  -  left. assumption.
+  - right.
+    s_struct.
+    destruct p; trivial.
+    unfold Q_and in Workie.
+    specialize (Workie Γ0 (A0 ∧ B) Γ').
+    simpl in Workie.
+    assert (Γ = Γ0 ++ [A0 ∧ B] ++ Γ').
+    {
+      auto.
+    }
+    symmetry in H.
+    simpl in H.
+    apply (Workie H A0 B).
+    + reflexivity.
+    + simpl in p.
+      assumption.
+Defined.
+
+
+
+
+
+Definition Q_or (A : formula)  (l0 : list formula) (A0 : formula) (l1 : list formula) :=
+  (forall B C, A0 = (B ∨ C) -> ( notT (l0 ++ [B] ++ l1 ⊢ A)) \/ ( notT  (l0 ++ [C] ++ l1 ⊢ A) )).
+
+Lemma f_or : forall  l0 A0 l1, l0 ++ [A0] ++ l1= Γ -> (Γ ⊢ A) + { Q_or A l0 A0 l1 }.
+Proof.
+  intros l0 A0 l1 eq.
+  unfold Q_or.
+  specialize (decidable_or A0) as [[[B C] eq0] | Neg].
+  - specialize (deg_IE_or_left l0 B C l1 A) as Deg_left.
+    specialize (deg_IE_or_right l0 B C l1 A) as Deg_right.
+    rewrite eq0 in eq.
+    rewrite <- eq in IH.
+    apply IH in Deg_left, Deg_right.
+    destruct Deg_left as [L | R]; destruct Deg_right as [LL | RR].
+    + rewrite <- eq.
+      left.
+      apply IE_or; assumption.
+    + right.
+      destruct S.
+      intros B0 C0 H.
+      right.
+      rewrite H in eq0.
+      inversion eq0.
+      subst.
       assumption.
     + right.
-      intro p.
-      assert (S = (Γ ⊢? A)) as S_struct.
-      {
-        destruct S. reflexivity.
-      }
-      destruct p; trivial.
-      apply Bad.
-      rewrite <- eq_Γ in S_struct.
-      inversion S_struct.
-      assert (Γ0 = l /\ Γ' = r).
-      {
-        split.
-        * induction l.
-      }
-      
-    
+      intros B0 C0 H.
+      subst.
+      inversion H.
+      left.
+      rewrite <- H1.
+      assumption.
+    + right.
+      intros B0 C0 H.
+      subst.
+      inversion H.
+      subst.
+      left.
+      assumption.
+  - right.
+    intros B C H.
+    subst.
+    specialize (Neg B C) as K.
+    contradiction.
+Defined.
 
+Lemma pre_IE_or : (Γ ⊢ A) + {
+      forall l0 A0 l1, l0 ++ [A0] ++ l1 = Γ -> Q_or A l0 A0 l1}.
+Proof.
+  specialize (list_split_ind  formula (Γ ⊢ A)  (Q_or A) Γ f_or) as [Fine | NotFine].
+  - left. assumption.
+  - right.
+    intros l0 A0 l1 H.
+    apply NotFine.
+    assumption.
+Defined.
+
+  
+
+  
+
+Lemma provable_with_IE_or :
+   (Γ ⊢ A) +
+  { forall (p : LI S),
+        match p with
+        | IE_or _  _ => False
+        | _ => True
+        end
+  }.
+Proof.
+  specialize pre_IE_or as [Done | Workie].
+  -  left. assumption.
+  - right.
+    s_struct.
+    destruct p; trivial.
+    unfold Q_or in Workie.
+    specialize (Workie Γ0 (A0 ∨ B) Γ').
+    simpl in Workie.
+    assert (Γ = Γ0 ++ [A0 ∨ B] ++ Γ').
+    {
+      auto.
+    }
+    symmetry in H.
+    simpl in H.
+    specialize (Workie H A0 B).
+    assert (A0 ∨ B = A0 ∨ B).
+    { reflexivity. }
+    apply Workie in H0.
+    destruct H0 as [L | R].
+    + apply L. simpl in p1. assumption.
+    + apply R. simpl in p2. assumption.
+Defined.
+
+
+
+Definition Q_impl_and (A : formula)  (l0 : list formula) (A0 : formula) (l1 : list formula) :=
+  (forall B C D, A0 = ((B ∧ C) ⇒ D )-> notT (l0 ++ [B ⇒ C ⇒ D] ++ l1 ⊢ A)).
+
+Lemma f_impl_and : forall  l0 A0 l1, l0 ++ [A0] ++ l1= Γ -> (Γ ⊢ A) + { Q_impl_and A l0 A0 l1 }.
+Proof.
+  intros l0 A0 l1 eq.
+  unfold Q_impl_and.
+  specialize (decidable_impl_and A0) as [[[[B C] D] eq0] | Neg].
+  - specialize (deg_IE_impl_and l0 B C D l1 A) as Deg.
+    rewrite eq0 in eq.
+    rewrite <- eq in IH.
+    apply IH in Deg.
+    destruct Deg as [L | R].
+    + rewrite <- eq.
+      left.
+      apply IE_impl_and; assumption.
+    + right.
+      destruct S.
+      intros B0 C0 D0 H.
+      rewrite H in eq0.
+      inversion eq0.
+      subst.
+      assumption.
+  - right.
+    intros B C D H.
+    subst.
+    specialize (Neg B C D) as K.
+    contradiction.
+Defined.
+
+Lemma pre_IE_impl_and : (Γ ⊢ A) + {
+      forall l0 A0 l1, l0 ++ [A0] ++ l1 = Γ -> Q_impl_and A l0 A0 l1}.
+Proof.
+  specialize (list_split_ind  formula (Γ ⊢ A)  (Q_impl_and A) Γ f_impl_and) as [Fine | NotFine].
+  - left. assumption.
+  - right.
+    intros l0 A0 l1 H.
+    apply NotFine.
+    assumption.
+Defined.
+
+Lemma provable_with_IE_impl_and :
+   (Γ ⊢ A) +
+  { forall (p : LI S),
+        match p with
+        | IE_impl_and _ => False
+        | _ => True
+        end
+  }.
+Proof.
+  specialize pre_IE_impl_and as [Done | Workie].
+  -  left. assumption.
+  - right.
+    s_struct.
+    destruct p; trivial.
+    unfold Q_impl_and in Workie.
+    specialize (Workie Γ0 ((A0 ∧ B) ⇒ C) Γ').
+    simpl in Workie.
+    assert (Γ = Γ0 ++ [(A0 ∧ B) ⇒ C] ++ Γ').
+    {
+      auto.
+    }
+    symmetry in H.
+    simpl in H.
+    apply (Workie H A0 B C).
+    + reflexivity.
+    + simpl in p.
+      assumption.
+Defined.
+
+Definition Q_impl_or (A : formula)  (l0 : list formula) (A0 : formula) (l1 : list formula) :=
+  (forall B C D, A0 = ((B ∨ C) ⇒ D )-> notT (l0 ++ [B ⇒ D] ++ [C ⇒ D] ++ l1 ⊢ A)).
+
+Lemma f_impl_or : forall  l0 A0 l1, l0 ++ [A0] ++ l1= Γ -> (Γ ⊢ A) + { Q_impl_or A l0 A0 l1 }.
+Proof.
+  intros l0 A0 l1 eq.
+  unfold Q_impl_or.
+  specialize (decidable_impl_or A0) as [[[[B C] D] eq0] | Neg].
+  - specialize (deg_IE_impl_or l0 B C D l1 A) as Deg.
+    rewrite eq0 in eq.
+    rewrite <- eq in IH.
+    apply IH in Deg.
+    destruct Deg as [L | R].
+    + rewrite <- eq.
+      left.
+      apply IE_impl_or; assumption.
+    + right.
+      destruct S.
+      intros B0 C0 D0 H.
+      rewrite H in eq0.
+      inversion eq0.
+      subst.
+      assumption.
+  - right.
+    intros B C D H.
+    subst.
+    specialize (Neg B C D) as K.
+    contradiction.
+Defined.
+
+Lemma pre_IE_impl_or : (Γ ⊢ A) + {
+      forall l0 A0 l1, l0 ++ [A0] ++ l1 = Γ -> Q_impl_or A l0 A0 l1}.
+Proof.
+  specialize (list_split_ind formula (Γ ⊢ A)  (Q_impl_or A) Γ f_impl_or) as [Fine | NotFine].
+  - left. assumption.
+  - right.
+    intros l0 A0 l1 H.
+    apply NotFine.
+    assumption.
+Defined.
+
+Lemma provable_with_IE_impl_or :
+   (Γ ⊢ A) +
+  { forall (p : LI S),
+        match p with
+        | IE_impl_or _ => False
+        | _ => True
+        end
+  }.
+Proof.
+  specialize pre_IE_impl_or as [Done | Workie].
+  -  left. assumption.
+  - right.
+    s_struct.
+    destruct p; trivial.
+    unfold Q_impl_or in Workie.
+    specialize (Workie Γ0 ((A0 ∨ B) ⇒ C) Γ').
+    simpl in Workie.
+    assert (Γ = Γ0 ++ [(A0 ∨ B) ⇒ C] ++ Γ').
+    {
+      auto.
+    }
+    symmetry in H.
+    simpl in H.
+    apply (Workie H A0 B C).
+    + reflexivity.
+    + simpl in p.
+      assumption.
+Defined.
+
+Definition Q_impl_impl (A : formula)  (l0 : list formula) (A0 : formula) (l1 : list formula) :=
+  (forall B C D, A0 = ((B ⇒  C) ⇒ D )-> notT (l0 ++ [B; C ⇒ D] ++ l1 ⊢ A)).
+
+Lemma f_impl_impl : forall  l0 A0 l1, l0 ++ [A0] ++ l1= Γ -> (Γ ⊢ A) + { Q_impl_impl A l0 A0 l1 }.
+Proof.
+  intros l0 A0 l1 eq.
+  unfold Q_impl_impl.
+  specialize (decidable_impl_impl A0) as [[[[B C] D] eq0] | Neg].
+  - specialize (deg_IE_impl_impl_left l0 B C D l1 A) as Deg_left.
+    specialize (deg_IE_impl_impl_right l0 B C D l1 A) as Deg_right.
+    rewrite eq0 in eq.
+    rewrite <- eq in IH.
+    apply IH in Deg_left, Deg_right.
+    destruct Deg_left as [L | R]; destruct Deg_right as [LL | RR].
+    + rewrite <- eq.
+      left.
+      apply IE_impl_impl; assumption.
+    + right.
+      intros B0 C0 D0 H.
+      rewrite H in eq0.
+      inversion eq0.
+      subst.
+      admit.
+    + right.
+      intros B0 C0 D0 H.
+      subst.
+      inversion H.
+      subst.
+      admit.
+    + admit.
+  - right.
+    intros B C D H.
+    subst.
+    specialize (Neg B C D) as K.
+    contradiction.
+Admitted.
+
+
+Lemma pre_IE_impl_impl : (Γ ⊢ A) + {
+      forall l0 A0 l1, l0 ++ [A0] ++ l1 = Γ -> Q_impl_impl A l0 A0 l1}.
+Proof.
+  specialize (list_split_ind  formula (Γ ⊢ A)  (Q_impl_impl A) Γ f_impl_impl) as [Fine | NotFine].
+  - left. assumption.
+  - right.
+    intros l0 A0 l1 H.
+    apply NotFine.
+    assumption.
+Defined.
+
+Lemma provable_with_IE_impl_impl :
+   (Γ ⊢ A) +
+  { forall (p : LI S),
+        match p with
+        | IE_impl_impl _ _ => False
+        | _ => True
+        end
+  }.
+Proof.
+  specialize pre_IE_impl_impl as [Done | Workie].
+  -  left. assumption.
+  - right.
+    s_struct.
+    destruct p; trivial.
+    unfold Q_impl_impl in Workie.
+    specialize (Workie Γ0 ((A0 ⇒ B) ⇒ C) Γ').
+    simpl in Workie.
+    assert (Γ = Γ0 ++ [(A0 ⇒ B) ⇒ C] ++ Γ').
+    {
+      auto.
+    }
+    symmetry in H.
+    simpl in H.
+    apply (Workie H A0 B C).
+    + reflexivity.
+    + admit.
+Admitted.
+
+
+(*
+Lemma pre_IE_impl_left : (Γ ⊢ A) + {
+      forall l0 A0 l1, l0 ++ [A0] ++ l1 = Γ -> Q_impl_left A l0 A0 l1}.
+Proof.
+  specialize (list_split_ind  formula (Γ ⊢ A)  (Q_impl_left A) Γ f_impl_left) as [Fine | NotFine].
+  - left. assumption.
+  - right.
+    intros l0 A0 l1 H.
+    apply NotFine.
+    assumption.
+Defined.
+*)
+
+Lemma provable_with_IE_impl_left :
+   (Γ ⊢ A) +
+  { forall (p : LI S),
+        match p with
+        | IE_impl_left _ _ => False
+        | _ => True
+        end
+  }.
+Proof.
 
 Admitted.
 
